strcmp.dfy
@@ -1,60 +1,118 @@
 function method min(a: int, b: int): int
 { if a <= b then a else b }
 
+predicate PrecedeEqual(a: array<char>, b: array<char>, n: int)
+requires 0 <= n <= min(a.Length, b.Length);
+reads a, b;
+{ forall i :: 0 <= i < n ==> a[i] == b[i] }
+
+predicate StringLessThan(a: array<char>, b: array<char>)
+requires a.Length > 0 && b.Length > 0;
+reads a, b;
+{ exists k :: 0 <= k < min(a.Length, b.Length) && a[k] < b[k] && PrecedeEqual(a, b, k) }
+
+predicate StringMoreThan(a: array<char>, b: array<char>)
+requires a.Length > 0 && b.Length > 0;
+reads a, b;
+{ exists k :: 0 <= k < min(a.Length, b.Length) && a[k] > b[k] && PrecedeEqual(a, b, k) }
+
+method strcmp(a: array<char>, b: array<char>) returns (res: int)
+requires a.Length > 0 && b.Length > 0;
+ensures res == 0 || res == 1 || res == -1;
+ensures res == 0  ==> a.Length == b.Length && PrecedeEqual(a, b, a.Length);
+ensures res == -1 ==> StringLessThan(a, b) || (a.Length < b.Length && PrecedeEqual(a, b, a.Length));
+ensures res == 1  ==> StringMoreThan(a, b) || (a.Length > b.Length && PrecedeEqual(a, b, b.Length));
+{
+    var i := 0;
+    res := 0;
+    var minLen := min(a.Length, b.Length);
+    while (i < minLen)
+    invariant 0 <= i <= min(a.Length, b.Length);
+    invariant PrecedeEqual(a, b, i);
+    {
+        if (a[i] < b[i]) { return -1; }
+        else if (a[i] > b[i]) { return 1; }
+        i := i + 1;
+    }
+    
+    if (a.Length < b.Length) { return -1; }
+    else if (a.Length > b.Length) { return 1; }
+    else if (a.Length == b.Length) { return 0; }
+}
+
+method Main() {
+  var a :array<char> := new char[5];
+  a[0], a[1], a[2], a[3], a[4] := 'h', 'e', 'l', 'l', 'o';
+  var b :array<char> := new char[4];
+  b[0], b[1], b[2], b[3] := 'h', 'e', 'l', 'l';
+  var c :array<char> := new char[4];
+  c[0], c[1], c[2], c[3] := 'w', 'h', 'a', 't';
+  
+  var cmp := strcmp(a, a);
+  assert cmp == 0;
+  
+  cmp := strcmp(a, b);
+  assert cmp == 1;
+  
+  cmp := strcmp(b, a);
+  assert cmp == -1;
+  
+  assert a[0] == 'h'; assert a[1] == 'e'; assert a[2] == 'l'; assert a[3] == 'l'; assert a[4] == 'o';
+  assert b[0] == 'h'; assert b[1] == 'e'; assert b[2] == 'l'; assert b[3] == 'l';
+  assert c[0] == 'w'; assert c[1] == 'h'; assert c[2] == 'a'; assert c[3] == 't';
+  cmp := strcmp(a, c);
+  assert cmp == -1;
+  
+  cmp := strcmp(c, a);
+  assert cmp == 1;
+  
+  cmp := strcmp(b, c);
+  assert cmp == -1;
+  
+  cmp := strcmp(c, b);
+  assert cmp == 1;
+}
+
+/* NOT VERIFY FOR STRING/SEQ<CHAR>
+function method min(a: int, b: int): int
+{ if a <= b then a else b }
+
 predicate PrecedeEqual(a: string, b: string, n: int)
 requires 0 <= n <= min(|a|, |b|);
 { forall i :: 0 <= i < n ==> a[i] == b[i] }
 
-predicate StringLessThan(a: string, b:string)
+predicate StringLessThan(a: string, b: string)
 requires |a| > 0 && |b| > 0;
 { exists k :: 0 <= k < min(|a|, |b|) && a[k] < b[k] && PrecedeEqual(a, b, k) }
 
-predicate StringMoreThan(a: string, b:string)
+predicate StringMoreThan(a: string, b: string)
 requires |a| > 0 && |b| > 0;
 { exists k :: 0 <= k < min(|a|, |b|) && a[k] > b[k] && PrecedeEqual(a, b, k) }
-
-//predicate StringEqual(a: string, b: string)
-//{ |a| == |b| && PrecedeEqual(a, b, |a|) }
 
 method strcmp(a: string, b: string) returns (res: int)
 requires |a| > 0 && |b| > 0;
 ensures res == 0 || res == 1 || res == -1;
-ensures res == 0  <==> a == b;
-ensures res == -1 <==> StringLessThan(a, b) || (|a| < |b| && PrecedeEqual(a, b, |a|));
-ensures res == 1  <==> StringMoreThan(a, b) || (|a| > |b| && PrecedeEqual(a, b, |b|));
+ensures res == 0  ==> |a| == |b| && PrecedeEqual(a, b, |a|);
+ensures res == -1 ==> StringLessThan(a, b) || (|a| < |b| && PrecedeEqual(a, b, |a|));
+ensures res == 1  ==> StringMoreThan(a, b) || (|a| > |b| && PrecedeEqual(a, b, |b|));
 {
     var i := 0;
+    res := 0;
     var minLen := min(|a|, |b|);
-    while (i < minLen)
+    while (i < minLen && res == 0)
     invariant 0 <= i <= min(|a|, |b|);
-    invariant PrecedeEqual(a, b, i);
+    invariant res == 0  ==> PrecedeEqual(a, b, i);
+    invariant res == 1  ==> StringMoreThan(a, b);
+    invariant res == -1 ==> StringLessThan(a, b);
     {
-        if (a[i] < b[i]) { return -1; }
-        else if (a[i] > b[i]) {return 1; }
+        if (a[i] < b[i]) { res := -1; }
+        else if (a[i] > b[i]) { res := 1; }
         i := i + 1;
     }
-    assert PrecedeEqual(a, b, min(|a|, |b|));
+    if (res != 0) { return res; }
+    
     if (|a| < |b|) { return -1; }
     else if (|a| > |b|) { return 1; }
     else if (|a| == |b|) { return 0; }
 }
-
-method Main() {
-  var a := "hello";
-  var b := "what";
-  var c := "hello";
-  
-  assert a == c;
-  var cmp := strcmp(a, c);
-  assert cmp == 0;
-  
-  assert a == "hello" && b == "what";
-  cmp := strcmp(a, b);
-  print "strcmp(", a, ",", b, ")=", cmp, '\n';
-  assert cmp == -1;
-  
-  assert a == "hello" && b == "what";
-  cmp := strcmp(b, a);
-  print "strcmp(", b, ",", a, ")=", cmp, '\n';
-  assert cmp == 1;
-}
+*/
